src/ExpansionScript.sml
@@ -11,9 +11,7 @@
 open HolKernel Parse boolLib bossLib;
 
 open relationTheory listTheory;
-open CCSLib CCSTheory;
-open StrongEQTheory StrongLawsTheory;
-open WeakEQTheory WeakLawsTheory;
+open CCSLib CCSTheory StrongEQTheory StrongLawsTheory WeakEQTheory WeakLawsTheory;
 open CongruenceTheory TraceTheory;
 
 val _ = new_theory "Expansion";
